src/proof/controllers/replicaset.v
@@ -19,13 +19,75 @@ Definition current_state_matches rs pods : Prop :=
   | None => False
   end.
 
+Lemma lookup_filter_ge {A} (P : A → Prop) `{∀ x, Decision (P x)}
+    (l : list A) (n : nat) x :
+  filter P l !! n = Some x →
+  ∃ k : nat, n ≤ k ∧ l !! k = Some x.
+Proof.
+  revert n.
+  induction l as [|y l IH]; intros n Hlookup.
+  - destruct n; inversion Hlookup.
+  - rewrite filter_cons in Hlookup.
+    destruct (decide (P y)) as [Hy|Hy].
+    + destruct n as [|n].
+      * simpl in Hlookup. inversion Hlookup; subst.
+        exists O. split; done.
+      * simpl in Hlookup.
+        destruct (IH n Hlookup) as (k & Hle & Hk).
+        exists (S k). split; [lia|done].
+    + destruct (IH n Hlookup) as (k & Hle & Hk).
+      exists (S k). split; [lia|done].
+Qed.
+
+Lemma lookup_filter_elem_of_drop {A} (P : A → Prop) `{∀ x, Decision (P x)}
+    (l : list A) (n : nat) x :
+  filter P l !! n = Some x →
+  x ∈ drop n l.
+Proof.
+  intros Hlookup.
+  destruct (lookup_filter_ge P l n x Hlookup) as (k & Hle & Hk).
+  apply (list_elem_of_lookup_2 (drop n l) (k - n) x).
+  rewrite lookup_drop.
+  replace (n + (k - n))%nat with k by lia.
+  done.
+Qed.
+
+Lemma take_drop_middle_slices {A} (l : list A) i x :
+  l !! i = Some x →
+  take i l = take i (take i l ++ x :: drop (S i) l) ∧
+  drop (S i) (take i l ++ x :: drop (S i) l) = drop (S i) l.
+Proof.
+  intros Hlookup.
+  pose proof (lookup_lt_Some _ _ _ Hlookup) as Hlt.
+  split.
+  - assert ((i <= length (take i l))%nat) as Hlen_take by (rewrite length_take_le; lia).
+    rewrite (take_app_le (take i l) (x :: drop (S i) l) i Hlen_take).
+    rewrite take_take Nat.min_id. done.
+  - replace (S i) with (length (take i l) + 1)%nat by (rewrite length_take_le; lia).
+    rewrite drop_app_add. done.
+Qed.
+
+Lemma big_sepL_split_lookup {A} (Φ : A → iProp Σ) (l : list A) i x :
+  l !! i = Some x →
+  ([∗ list] y ∈ l, Φ y) -∗
+  ([∗ list] y ∈ take i l, Φ y) ∗ Φ x ∗ ([∗ list] y ∈ drop (S i) l, Φ y).
+Proof.
+  iIntros (Hlookup) "H".
+  destruct (take_drop_middle_slices l i x Hlookup) as [Htake Hdrop].
+  rewrite -(take_drop_middle l i x Hlookup) big_sepL_app /=.
+  iDestruct "H" as "(Hbefore & Hx & Hafter)".
+  iEval (rewrite Htake) in "Hbefore".
+  iEval (rewrite -Hdrop) in "Hafter".
+  iFrame.
+Qed.
+
 Lemma wp_manageReplicas γ l (gv: schema.GroupVersion.t) sl rs_l ptrs pods rs n dq1 dq2 :
   {{{ is_pkg_init code.controllers.replicaset.replicaset ∗
       "#Hisk" ∷ is_kubernetes γ l ∗
       "#Hglobal_l" ∷ (global_addr common.State) ↦□ l ∗
       "#Hglobal_gv" ∷ (global_addr v1.SchemeGroupVersion) ↦□ gv ∗
       "Hsl" ∷ sl ↦* ptrs ∗
-      "Hdeepown_l_pods" ∷ ([∗ list] ptr;pod ∈ ptrs;pods, PodV.deepown_l ptr pod dq1) ∗
+      "Hdeepown_l_pods" ∷ ([∗ list] ptr;pod ∈ ptrs;filter is_pod_alive pods, PodV.deepown_l ptr pod dq1) ∗
       "Hdeepown_l_rs" ∷ ReplicaSetV.deepown_l rs_l rs dq2 ∗
       "Hown_pod_meta_frags" ∷ ([∗ list] pod ∈ pods,
         own_meta_frag γ (PodV.key pod) pod.(PodV.ObjectMeta').(ObjectMetaV.UID') 1 pod.(PodV.ObjectMeta')) ∗
@@ -33,15 +95,13 @@ Lemma wp_manageReplicas γ l (gv: schema.GroupVersion.t) sl rs_l ptrs pods rs n 
         rs.(ReplicaSetV.ObjectMeta').(ObjectMetaV.UID') 1 (list_to_set (PodV.key <$> pods)) ∗
       "%Hrs_valid" ∷ ⌜ ReplicaSetV.valid rs ⌝ ∗
       "%Hrs_name_short" ∷ ⌜ length rs.(ReplicaSetV.ObjectMeta').(ObjectMetaV.Name') < 58 ⌝ ∗
-      "%Hpods_active" ∷ ⌜ Forall is_pod_alive pods ⌝ ∗
       "%Hreplicas_eq" ∷ ⌜ rs.(ReplicaSetV.Spec').(ReplicaSetSpecV.Replicas') = Some n ⌝
   }}}
     @! replicaset.manageReplicas #sl #rs_l
   {{{ pods', RET #interface.nil;
-      ⌜ length pods' = sint.nat n ⌝ ∗
-      ⌜ Forall is_pod_alive pods' ⌝ ∗
+      ⌜ length (filter is_pod_alive pods') = sint.nat n ⌝ ∗
       sl ↦* ptrs ∗
-      ([∗ list] ptr;pod ∈ ptrs;pods, PodV.deepown_l ptr pod dq1) ∗
+      ([∗ list] ptr;pod ∈ ptrs;filter is_pod_alive pods, PodV.deepown_l ptr pod dq1) ∗
       ReplicaSetV.deepown_l rs_l rs dq2 ∗
       ([∗ list] pod ∈ pods',
         own_meta_frag γ (PodV.key pod) pod.(PodV.ObjectMeta').(ObjectMetaV.UID') 1 pod.(PodV.ObjectMeta')) ∗
@@ -74,12 +134,11 @@ Proof.
         own_meta_frag γ (PodV.key pod) pod.(PodV.ObjectMeta').(ObjectMetaV.UID') 1 pod.(PodV.ObjectMeta')) ∗
       "Hown_children_frag" ∷ own_children_frag γ (ReplicaSetV.key rs)
         rs.(ReplicaSetV.ObjectMeta').(ObjectMetaV.UID') 1 (list_to_set (PodV.key <$> pods')) ∗
-      "%Hpods_active'" ∷ ⌜ Forall is_pod_alive pods' ⌝ ∗
-      "%Hlength_eq'" ∷ ⌜ length pods' = Z.to_nat ((sint.Z (slice.len_f sl)) + sint.Z i) ⌝ ∗
+      "%Hpod_number'" ∷ ⌜ length (filter is_pod_alive pods') = Z.to_nat ((sint.Z (slice.len_f sl)) + sint.Z i) ⌝ ∗
       "%Hi" ∷ ⌜ 0 ≤ sint.Z i ≤ sint.Z (word.mul (word.sub (slice.len_f sl) (W64 (sint.Z n))) (W64 (-1))) ⌝
     )%I.
     iAssert (I) with "[i Hown_pod_meta_frags Hown_children_frag]" as "Hloop_inv".
-    { iExists (W64 0), pods. iFrame. iPureIntro. split_and!; [done|word|word|word]. }
+    { iExists (W64 0), pods. iFrame. iPureIntro. split_and!; word. }
     wp_for "Hloop_inv". wp_if_destruct.
     + wp_apply wp_globals_get. wp_apply schema.wp_GroupVersion__WithKind.
       { (* TODO: why? *) iAssert (is_pkg_init code.k8s_io.api.apps.v1.v1) as "H". all: iPkgInit. }
@@ -115,29 +174,139 @@ Proof.
         iSplitL "Hown_pod_meta_frags Hcreate_Hown_meta".
         - rewrite big_sepL_app. simpl. iFrame.
         - iSplitL "Hcreate_Hown_children".
-          + assert (list_to_set (PodV.key <$> pods') ∪ {[PodV.key pod']} = list_to_set (PodV.key <$> pods' ++ [pod']))
-              as ->.
-            { rewrite fmap_app. set_solver. }
-            done.
-          + iPureIntro.
-            split_and!.
-            * rewrite Forall_app. split; [done|].
-              constructor; [|constructor].
-              unfold is_pod_alive.
-              unfold ObjectMetaV.nameless_created in Hcreate_Hmeta_created.
-              naive_solver.
-            * rewrite app_length /= Hlength_eq'.
-              word.
-            * word.
-            * word.
+            + assert (list_to_set (PodV.key <$> pods') ∪ {[PodV.key pod']} = list_to_set (PodV.key <$> pods' ++ [pod']))
+                as ->.
+              { rewrite fmap_app. set_solver. }
+              done.
+            + iPureIntro.
+              split_and!.
+              * assert (length (filter is_pod_alive (pods' ++ [pod'])) =
+                  S (length (filter is_pod_alive pods'))) as Hfilter_len.
+                { assert (is_pod_alive pod') as Hpod_alive.
+                  { unfold is_pod_alive.
+                    unfold ObjectMetaV.nameless_created in Hcreate_Hmeta_created.
+                    naive_solver.
+                  }
+                  clear -Hpod_alive.
+                  induction pods' as [|pod0 pods'' IH]; simpl.
+                  - rewrite filter_cons.
+                    rewrite decide_True; done.
+                  - rewrite !filter_cons.
+                    destruct (decide (is_pod_alive pod0)); simpl.
+                    + f_equal. exact IH.
+                    + exact IH.
+                }
+                rewrite Hfilter_len Hpod_number'.
+                word.
+              * word.
+              * word.
       }
       iFrame. iApply (struct_fields_combine (V:=v1.ReplicaSetSpec.t)). iFrame.
-    + iApply "HΦ". iFrame. iSplitR. 1: iPureIntro; word. iSplitR. 1: done.
+    + iApply "HΦ". iFrame. iSplitR. 1: iPureIntro; word.
       iApply ReplicaSetV.deepown_l_restore. iFrame.
       iSplitR. 1: done. iSplitL. 2: done.
       rewrite Hreplicas_eq. iExists n. iSplitL. all: done.
-  - admit.
-Admitted.
+  - wp_if_destruct.
+    2 : { iApply "HΦ". iFrame.
+      iSplit. 1: iPureIntro; word.
+      iApply ReplicaSetV.deepown_l_restore. iFrame.
+      iSplitR. 1: done. iSplitL. 2: done.
+      rewrite Hreplicas_eq. iExists n. iSplitL. all: done. }
+    wp_apply wp_slice_slice_pure; [iPureIntro;word|].
+    iDestruct (own_slice_f 0 (word.sub (slice.len_f sl) (W64 (sint.Z n))) with "Hsl")
+      as "(Hbefore_slice & Hslice & Hafter_slice )"; [word|].
+    iDestruct (own_slice_len with "Hslice") as %(Hslice_len1 & Hslice_len2).
+    set I := (∃ (i: w64) (pod_l: loc) (pods': list PodV.t),
+      "Hi_ptr" ∷ i_ptr ↦ i ∗
+      "Hpod_ptr" ∷ pod_ptr ↦ pod_l ∗
+      "Hown_pod_meta_frags" ∷ ([∗ list] pod ∈ pods',
+        own_meta_frag γ (PodV.key pod) pod.(PodV.ObjectMeta').(ObjectMetaV.UID') 1 pod.(PodV.ObjectMeta')) ∗
+      "Hown_children_frag" ∷ own_children_frag γ (ReplicaSetV.key rs)
+        rs.(ReplicaSetV.ObjectMeta').(ObjectMetaV.UID') 1 (list_to_set (PodV.key <$> pods')) ∗
+      "%Hincluded" ∷ ⌜ ∀ pod, pod ∈ drop (sint.nat i) pods → pod ∈ pods' ⌝ ∗
+      "%Hlength" ∷ ⌜ length (filter is_pod_alive pods') = Z.to_nat ((sint.Z (slice.len_f sl)) - sint.Z i) ⌝ ∗
+      "%Hi" ∷ ⌜ 0 ≤ sint.Z i ≤ sint.Z (slice.len_f (slice.slice_f sl ptrT (W64 0) (word.sub (slice.len_f sl) (W64 (sint.Z n))))) ⌝
+    )%I.
+    iAssert (I) with "[i pod Hown_pod_meta_frags Hown_children_frag]" as "Hloop_inv".
+    { iExists (W64 0), (default_val loc), pods. iFrame. iPureIntro. split_and!.
+      - rewrite drop_0. done.
+      - word.
+      - word.
+      - word.
+    }
+    wp_for "Hloop_inv". wp_if_destruct.
+    + wp_pure; [rewrite /slice.slice_f /=;word|].
+      set sliced_ptrs := (subslice (sint.nat (W64 0)) (sint.nat (word.sub (slice.len_f sl) (W64 (sint.Z n)))) ptrs).
+      list_elem sliced_ptrs (sint.Z i) as this_ptr.
+      { rewrite Hslice_len1 /slice.slice_f /=. word. }
+      wp_apply (wp_load_slice_elem with "[$Hslice]"); [word|eauto|].
+      iIntros "Hslice". wp_auto.
+      assert (ptrs !! sint.nat i = Some this_ptr) as Hlookup_ptrs.
+      { eapply lookup_take_Some in Hthis_ptr_lookup. intuition. }
+      assert (∃ this_pod, (filter is_pod_alive pods) !! sint.nat i = Some this_pod) as [this_pod Hlookup_active_pods].
+      { apply lookup_lt_is_Some_2. rewrite <-Hlen. word. }
+      iDestruct (big_sepL2_lookup_acc with "Hdeepown_l_pods") as "[Hdeepown_l_this Hdeepown_l_others]".
+      { apply Hlookup_ptrs. }
+      { apply Hlookup_active_pods. }
+      iPoseProof (PodV.deepown_l_split with "Hdeepown_l_this") as
+        "(Hdeepown_t_l_pod & Hdeepown_m_l_pod & Hdeepown_s_l_pod & Hdeepown_st_l_pod)".
+      wp_apply (v1.wp_GetUID_deepown with "[$Hdeepown_m_l_pod]"). iIntros "Hdeepown_m_l_pod". wp_auto.
+      wp_apply (v1.wp_GetNamespace_deepown with "[$Hdeepown_m_l_pod]"). iIntros "Hdeepown_m_l_pod". wp_auto.
+      wp_apply (v1.wp_GetName_deepown with "[$Hdeepown_m_l_pod]"). iIntros "Hdeepown_m_l_pod". wp_auto.
+      wp_apply (common.wp_NewDeleteOptionsWithUID). iIntros (do_c) "(Hdeepown_do & %Hvalid_do)". wp_auto.
+      wp_apply wp_globals_get.
+      assert (∃ j, pods' !! j = Some this_pod) as [j Hlookup_pods'].
+      { apply list_elem_of_lookup_1, Hincluded.
+        eapply lookup_filter_elem_of_drop.
+        exact Hlookup_active_pods. }
+      iPoseProof (big_sepL_split_lookup _ _ _ _ Hlookup_pods' with "Hown_pod_meta_frags") as
+        "(Hown_pod_meta_frags_before & Hown_pod_meta_frag_this & Hown_pod_meta_frags_after)".
+      wp_apply (wp_State__PodDelete_matching_pre with "[$Hdeepown_do $Hown_pod_meta_frag_this $Hown_children_frag]").
+      { iFrame "#". iSplit.
+        - iAssert (is_pkg_init code.controllers.common.common) as "H". all: iPkgInit.
+        - iPureIntro. split_and!. all: try done.
+          rewrite elem_of_list_to_set.
+          apply list_elem_of_fmap_2.
+          eapply list_elem_of_lookup_2.
+          exact Hlookup_pods'. }
+      iIntros (kmeta') "H". wp_auto.
+      rewrite bool_decide_true //. wp_auto.
+      iApply wp_for_post_do. wp_auto.
+      iDestruct "H" as "[H | H]".
+      * iNamedPrefix "H" "Hdelete_".
+        iAssert (I) with "[Hi_ptr Hpod_ptr Hown_pod_meta_frags_before Hown_pod_meta_frags_after Hdelete_Hown_meta_frag
+          Hdelete_Hown_children_frag]" as "loop_inv".
+	        { iExists (word.add i (W64 1)), this_ptr,
+	            (take j pods' ++ [this_pod <|PodV.ObjectMeta':=kmeta'|>] ++ drop (S j) pods').
+	          iPoseProof (kview.own_meta_valid with "Hdelete_Hown_meta_frag") as "%Hmeta_valid".
+	          destruct Hmeta_valid as (Hname_eq & Hnamespace_eq & Huid_eq & _).
+	          assert (PodV.key (this_pod <| PodV.ObjectMeta' := kmeta' |>) = PodV.key this_pod) as Hkey_eq.
+	          { rewrite /PodV.key /PodV.meta_key /=.
+	            rewrite -Hnamespace_eq -Hname_eq.
+	            done. }
+	          iFrame. iSplitL "Hdelete_Hown_meta_frag".
+	          { rewrite big_sepL_singleton Hkey_eq -Huid_eq. iFrame. }
+	          iSplitL.
+	          { assert (list_to_set (C:=gset KKey.t) (PodV.key <$>
+	              (take j pods' ++ [this_pod <| PodV.ObjectMeta' := kmeta' |>] ++ drop (S j) pods')) =
+	              list_to_set (C:=gset KKey.t) (PodV.key <$> pods')) as Hchildren_eq.
+	            { replace (list_to_set (C:=gset KKey.t) (PodV.key <$> pods')) with
+	                (list_to_set (C:=gset KKey.t)
+	                  (PodV.key <$> (take j pods' ++ [this_pod] ++ drop (S j) pods'))).
+	              2: { rewrite (take_drop_middle pods' j this_pod Hlookup_pods'). done. }
+	              rewrite !fmap_app /= Hkey_eq.
+	              done. }
+	            rewrite Hchildren_eq. iFrame. }
+		        iPureIntro. split_and!.
+	          - admit.
+	          - admit.
+            - word.
+            - rewrite /slice.slice_f /=. word.
+	        }
+        iFrame. iApply "Hdeepown_l_others".
+        (* iApply PodV.deepown_l_restore. iFrame. *)
+
+    Admitted.
 
 Lemma wp_syncReplicaSet γ l (gv: schema.GroupVersion.t) namespace name rs pods :
   {{{ is_pkg_init code.controllers.replicaset.replicaset ∗
